projects/PropositionalLogic/MetaTheorems.v
@@ -1,0 +1,1037 @@
+Require Import Coq.Arith.PeanoNat.
+Require Import Coq.Arith.Compare_dec.
+Require Import Coq.Lists.List.
+Require Import Coq.micromega.Lia.
+Require Import DschingisKhan.classical.ExclusiveMiddle.
+Require Import DschingisKhan.pure.CBA.
+Require Import DschingisKhan.pure.MyStructures.
+Require Import DschingisKhan.pure.MyUtilities.
+Require Import DschingisKhan.projects.PropositionalLogic.Basics.
+
+Module PropertiesOfPropostionalLogic.
+
+  Import ListNotations BasicSetoidTheory MyEnsemble BasicPosetTheory MyEnsembleNova CountableBooleanAlgebra SyntaxOfPL SemanticsOfPL InferenceRulesOfPL LindenbaumBooleanAlgebraOnPL.
+
+  Inductive TH : ensemble formula -> ensemble formula :=
+  | in_Theory :
+    forall hs : ensemble formula,
+    forall c : formula,
+    hs |- c ->
+    member c (TH hs)
+  .
+
+  Local Hint Constructors TH : core.
+
+  Local Instance formula_isCBA : @isCBA formula formula_isSetoid :=
+    LindenbaumBooleanAlgebra
+  .
+
+  Lemma lemma1_of_1_3_8 :
+    forall bs : ensemble formula,
+    isFilter (TH bs).
+  Proof with eauto with *.
+    intros bs.
+    split.
+    { exists (ImplicationF ContradictionF ContradictionF).
+      constructor.
+      apply ImplicationI.
+      apply ByAssumption...
+    }
+    split.
+    { intros b1 b2 H H0.
+      inversion H; subst.
+      constructor.
+      apply (cut_property b1).
+      - apply H1.
+      - apply (@extendInfers \left\{ b1 \right\} b2).
+        apply (proj1 (leq_LBA b1 b2) H0).
+        intros b.
+        rewrite in_insert_iff, in_singleton_iff...
+    }
+    { intros b1 b2 b H H0 [H1 H2].
+      inversion H; subst.
+      inversion H0; subst.
+      constructor.
+      apply (cut_property (ConjunctionF b1 b2)).
+      - apply ConjunctionI...
+      - apply (@extendInfers \left\{ andB b1 b2 \right\} b)...
+    }
+  Qed.
+
+  Local Hint Resolve lemma1_of_1_3_8 : core.
+
+  Lemma Cl_isSubsetOf_TH :
+    forall hs : ensemble formula,
+    isSubsetOf (Cl hs) (TH hs).
+  Proof with eauto with *.
+    intros hs.
+    enough ( claim1 :
+      forall ps : list formula,
+      (forall p : formula, In p ps -> member p hs) ->
+      forall c : formula,
+      andB (fold_right andB trueB ps) c == fold_right andB trueB ps ->
+      (exists hs' : ensemble formula, isSubsetOf hs' hs /\ hs' |- c)
+    ).
+    { intros p.
+      intro H.
+      inversion H; subst.
+      destruct (claim1 bs1 H0 p H1) as [hs' [H2 H3]].
+      constructor.
+      apply (extendInfers p H3)...
+    }
+    intros ps H c H0.
+    assert (H1 : \left\{ fold_right andB trueB ps \right\} |- c) by apply leq_LBA, H0.
+    destruct (proj1 (andBs_LBA ps hs H c) H1) as [hs' [H2 H3]].
+    exists hs'.
+    split...
+    intros h H4.
+    apply H.
+    apply H2...
+  Qed.
+
+  Local Hint Resolve Cl_isSubsetOf_TH : core.
+
+  Lemma infers_has_compactness :
+    forall hs : ensemble formula,
+    forall c : formula,
+    hs |- c ->
+    exists ps : list formula, (forall p : formula, In p ps -> member p hs) /\ (exists hs' : ensemble formula, (forall h : formula, In h ps <-> member h hs') /\ hs' |- c).
+  Proof with eauto with *.
+    intros hs c H.
+    induction H.
+    { exists (cons h nil).
+      split.
+      - intros p [H0 | []]; subst...
+      - exists (\left\{ h \right\}).
+        split.
+        + intros p.
+          split.
+          * intros [H0 | []]; subst...
+          * rewrite in_singleton_iff.
+            simpl...
+        + apply ByAssumption...
+    }
+    { destruct IHinfers1 as [ps1 [H1 [hs1' [H3 H5]]]].
+      destruct IHinfers2 as [ps2 [H2 [hs2' [H4 H6]]]].
+      exists (ps1 ++ ps2).
+      split.
+      - apply (in_append_implies ps1 ps2 hs H1 H2).
+      - exists (union hs1' hs2').
+        split.
+        + apply (in_append_iff ps1 ps2 hs1' hs2' H3 H4).
+        + apply (ContradictionI a).
+          * apply (extendInfers a H5)...
+          * apply (extendInfers (NegationF a) H6)...
+    }
+    { destruct IHinfers as [ps [H0 [hs' [H1 H2]]]].
+      exists ps...
+    }
+    { destruct IHinfers as [ps [H0 [hs' [H1 H2]]]].
+      exists (remove eq_formula_dec a ps).
+      split.
+      - apply in_remove_implies...
+      - exists (delete a hs').
+        split.
+        + apply in_remove_iff_member_delete...
+        + apply NegationI.
+          apply (extendInfers ContradictionF H2).
+          intros p H3.
+          destruct (eq_formula_dec p a) as [H_yes | H_no].
+          * subst...
+          * apply in_insert_iff, or_intror, in_delete_iff...
+    }
+    { destruct IHinfers as [ps [H0 [hs' [H1 H2]]]].
+      exists (remove eq_formula_dec (NegationF a) ps).
+      split.
+      - apply in_remove_implies...
+      - exists (delete (NegationF a) hs').
+        split.
+        + intros h.
+          apply (in_remove_iff_member_delete eq_formula_dec (NegationF a) ps hs' H1).
+        + apply NegationE.
+          apply (extendInfers ContradictionF H2).
+          intros h H3.
+          destruct (eq_formula_dec h (NegationF a)) as [H_yes | H_no].
+          * subst...
+          * apply in_insert_iff, or_intror, in_delete_iff...
+    }
+    { destruct IHinfers1 as [ps1 [H1 [hs1' [H3 H5]]]].
+      destruct IHinfers2 as [ps2 [H2 [hs2' [H4 H6]]]].
+      exists (ps1 ++ ps2).
+      split.
+      - apply (in_append_implies ps1 ps2 hs H1 H2).
+      - exists (union hs1' hs2').
+        split.
+        + apply (in_append_iff ps1 ps2 hs1' hs2' H3 H4).
+        + apply ConjunctionI.
+          * apply (extendInfers a H5)...
+          * apply (extendInfers b H6)...
+    }
+    { destruct IHinfers as [ps [H0 [hs' [H1 H2]]]].
+      exists ps...
+    }
+    { destruct IHinfers as [ps [H0 [hs' [H1 H2]]]].
+      exists ps...
+    }
+    { destruct IHinfers as [ps [H0 [hs' [H1 H2]]]].
+      exists ps...
+    }
+    { destruct IHinfers as [ps [H0 [hs' [H1 H2]]]].
+      exists ps...
+    }
+    { destruct IHinfers1 as [ps1 [H2 [hs1' [H5 H8]]]].
+      destruct IHinfers2 as [ps2 [H3 [hs2' [H6 H9]]]].
+      destruct IHinfers3 as [ps3 [H4 [hs3' [H7 H10]]]].
+      exists (ps1 ++ (remove eq_formula_dec a ps2 ++ remove eq_formula_dec b ps3)).
+      split.
+      - apply in_append_implies...
+        apply in_append_implies...
+        apply in_remove_implies...
+        apply in_remove_implies...
+      - exists (union hs1' (union (delete a hs2') (delete b hs3'))).
+        split.
+        { apply in_append_iff...
+          apply in_append_iff...
+          apply in_remove_iff_member_delete...
+          apply in_remove_iff_member_delete...
+        }
+        { apply (DisjunctionE a b c).
+          - apply (extendInfers (DisjunctionF a b) H8)...
+          - apply (extendInfers c H9).
+            intros p H11.
+            destruct (eq_formula_dec p a) as [H_yes | H_no].
+            + subst...
+            + apply in_insert_iff, or_intror, in_union_iff, or_intror, in_union_iff, or_introl, in_delete_iff...
+          - apply (extendInfers c H10).
+            intros p H11.
+            destruct (eq_formula_dec p b) as [H_yes | H_no].
+            + subst...
+            + apply in_insert_iff, or_intror, in_union_iff, or_intror, in_union_iff, or_intror, in_delete_iff...
+        }
+    }
+    { destruct IHinfers as [ps [H0 [hs' [H1 H2]]]].
+      exists (remove eq_formula_dec a ps).
+      split.
+      - apply in_remove_implies...
+      - exists (delete a hs').
+        split.
+        + apply in_remove_iff_member_delete...
+        + apply ImplicationI.
+          apply (extendInfers b H2).
+          intros p H3.
+          destruct (eq_formula_dec p a) as [H_yes | H_no].
+          * subst...
+          * apply in_insert_iff, or_intror, in_delete_iff...
+    }
+    { destruct IHinfers1 as [ps1 [H1 [hs1' [H3 H5]]]].
+      destruct IHinfers2 as [ps2 [H2 [hs2' [H4 H6]]]].
+      exists (ps1 ++ ps2).
+      split.
+      - apply (in_append_implies ps1 ps2 hs H1 H2).
+      - exists (union hs1' hs2').
+        split.
+        + apply (in_append_iff ps1 ps2 hs1' hs2' H3 H4).
+        + apply (ImplicationE a b).
+          * apply (extendInfers (ImplicationF a b) H5)...
+          * apply (extendInfers a H6)...
+    }
+    { destruct IHinfers1 as [ps1 [H1 [hs1' [H3 H5]]]].
+      destruct IHinfers2 as [ps2 [H2 [hs2' [H4 H6]]]].
+      exists (remove eq_formula_dec a ps1 ++ remove eq_formula_dec b ps2).
+      split.
+      - apply in_append_implies; apply in_remove_implies...
+      - exists (union (delete a hs1') (delete b hs2')).
+        split.
+        + apply in_append_iff; apply in_remove_iff_member_delete...
+        + apply BiconditionalI.
+          { apply (extendInfers b H5).
+            intros p H7.
+            destruct (eq_formula_dec p a) as [H_yes | H_no].
+            - subst...
+            - apply in_insert_iff, or_intror, in_union_iff, or_introl, in_delete_iff...
+          }
+          { apply (extendInfers a H6).
+            intros p H7.
+            destruct (eq_formula_dec p b) as [H_yes | H_no].
+            - subst...
+            - apply in_insert_iff, or_intror, in_union_iff, or_intror, in_delete_iff...
+          }
+    }
+    { destruct IHinfers1 as [ps1 [H1 [hs1' [H3 H5]]]].
+      destruct IHinfers2 as [ps2 [H2 [hs2' [H4 H6]]]].
+      exists (ps1 ++ ps2).
+      split.
+      - apply (in_append_implies ps1 ps2 hs H1 H2).
+      - exists (union hs1' hs2').
+        split.
+        + apply (in_append_iff ps1 ps2 hs1' hs2' H3 H4).
+        + apply (BiconditionalE1 a b).
+          * apply (extendInfers (BiconditionalF a b) H5)...
+          * apply (extendInfers a H6)...
+    }
+    { destruct IHinfers1 as [ps1 [H1 [hs1' [H3 H5]]]].
+      destruct IHinfers2 as [ps2 [H2 [hs2' [H4 H6]]]].
+      exists (ps1 ++ ps2).
+      split.
+      - apply (in_append_implies ps1 ps2 hs H1 H2).
+      - exists (union hs1' hs2').
+        split.
+        + apply (in_append_iff ps1 ps2 hs1' hs2' H3 H4).
+        + apply (BiconditionalE2 a b).
+          * apply (extendInfers (BiconditionalF a b) H5)...
+          * apply (extendInfers b H6)...
+    }
+  Qed.
+
+  Lemma TH_isSubsetOf_Cl :
+    forall hs : ensemble formula,
+    isSubsetOf (TH hs) (Cl hs).
+  Proof with eauto with *.
+    intros hs c H.
+    inversion H; subst.
+    destruct (infers_has_compactness hs c H0) as [ps [H1 H2]].
+    assert (claim1 := proj2 (andBs_LBA ps hs H1 c) H2).
+    exists ps.
+    - exact H1.
+    - apply leq_LBA...
+  Qed.
+
+  Lemma bound_exists :
+    forall ps : list formula,
+    exists bound : nat,
+    forall p : formula,
+    In p ps ->
+    exists n : nat, enum_formula n = p /\ n < bound.
+  Proof with lia || eauto with *.
+    induction ps as [| p ps [bound2 H]]; simpl.
+    - exists 0...
+    - destruct (formula_is_enumerable p) as [bound1 H0].
+      destruct (le_lt_dec bound1 bound2) as [Hle | Hlt].
+      + exists (S bound2).
+        intros h [H1 | H1].
+        * subst...
+        * destruct (H h H1) as [n [H2 H3]].
+          exists n...
+      + exists (S bound1).
+        intros h [H1 | H1].
+        * subst...
+        * destruct (H h H1) as [n [H2 H3]].
+          exists n...
+  Qed.
+
+  Definition Filter : ensemble formula -> nat -> ensemble formula :=
+    fun hs : ensemble formula =>
+    fun n : nat =>
+    improveFilter (TH hs) n
+  .
+
+  Definition AxmSet : ensemble formula -> nat -> ensemble formula :=
+    fun hs : ensemble formula =>
+    fix AxmSet_fix (n : nat) {struct n} : ensemble formula :=
+    match n with
+    | O => hs
+    | S n' => union (AxmSet_fix n') (insertion (Filter hs n') n')
+    end
+  .
+
+  Lemma property1_of_inconsistent :
+    forall hs : ensemble formula,
+    hs |- ContradictionF <-> inconsistent (Cl hs).
+  Proof with eauto with *.
+    intros hs.
+    split.
+    - intros H.
+      exists ContradictionF.
+      split...
+      apply TH_isSubsetOf_Cl...
+    - intros [b' [H [H0 H1]]].
+      assert (claim1 : member b' (TH hs)) by now apply (Cl_isSubsetOf_TH hs b' H).
+      inversion claim1; subst.
+      apply (cut_property b' ContradictionF).
+      + exact H2.
+      + apply (extendInfers ContradictionF H0)...
+  Qed.
+
+  Local Hint Resolve fact1_of_1_2_8 fact2_of_1_2_8 fact3_of_1_2_8 fact4_of_1_2_8 fact5_of_1_2_8 lemma1_of_1_2_11 inconsistent_isSubsetOf property1_of_inconsistent : core.
+
+  Lemma property1_of_equiconsistent :
+    forall hs1 : ensemble formula,
+    forall hs2 : ensemble formula,
+    isFilter hs1 ->
+    isFilter hs2 ->
+    equiconsistent hs1 hs2 <-> (hs1 |- ContradictionF <-> hs2 |- ContradictionF).
+  Proof with eauto with *.
+    intros hs1 hs2 HHH1 HHH2.
+    split.
+    - intros H.
+      split.
+      + intros H0.
+        apply property1_of_inconsistent.
+        apply (inconsistent_isSubsetOf hs2)...
+        apply H...
+        apply (inconsistent_isSubsetOf (Cl hs1))...
+        apply property1_of_inconsistent...
+      + intros H0.
+        apply property1_of_inconsistent.
+        apply (inconsistent_isSubsetOf hs1)...
+        apply H...
+        apply (inconsistent_isSubsetOf (Cl hs2))...
+        apply property1_of_inconsistent...
+    - intros H.
+      split.
+      + intros H0.
+        apply (inconsistent_isSubsetOf (Cl hs2))...
+        apply property1_of_inconsistent, H, property1_of_inconsistent...
+      + intros H0.
+        apply (inconsistent_isSubsetOf (Cl hs1))...
+        apply property1_of_inconsistent, H, property1_of_inconsistent...
+  Qed.
+
+  Lemma lemma1_of_1_3_9 :
+    forall n : nat,
+    forall hs : ensemble formula,
+    isSubsetOf (Filter hs n) (TH (AxmSet hs n)) /\ isSubsetOf (TH (AxmSet hs n)) (Filter hs n).
+  Proof with eauto with *.
+    unfold Filter.
+    induction n as [| n IH]; simpl.
+    - intros hs...
+    - intros hs.
+      destruct (IH hs) as [H H0].
+      assert (claim1 : isSubsetOf (Cl (union (improveFilter (TH hs) n) (insertion (improveFilter (TH hs) n) n))) (Cl (TH (union (AxmSet hs n) (insertion (Filter hs n) n))))).
+      { apply fact4_of_1_2_8.
+        intros b.
+        rewrite in_union_iff.
+        intro H1.
+        inversion H1; subst.
+        - assert (H3 := H b H2).
+          inversion H3; subst.
+          constructor.
+          apply (extendInfers b H4).
+          intros p H5.
+          apply in_union_iff, or_introl...
+        - constructor.
+          apply ByAssumption, in_union_iff, or_intror...
+      }
+      assert (claim2 : isSubsetOf (Cl (TH (union (AxmSet hs n) (insertion (Filter hs n) n)))) (TH (union (AxmSet hs n) (insertion (Filter hs n) n)))) by apply fact5_of_1_2_8, lemma1_of_1_3_8.
+      assert (claim3 : isSubsetOf (TH (union (AxmSet hs n) (insertion (Filter hs n) n))) (Cl (union (AxmSet hs n) (insertion (Filter hs n) n)))) by apply TH_isSubsetOf_Cl.
+      assert (claim4 : isSubsetOf (Cl (Cl (union (improveFilter (TH hs) n) (insertion (improveFilter (TH hs) n) n)))) (Cl (union (improveFilter (TH hs) n) (insertion (improveFilter (TH hs) n) n)))) by apply fact5_of_1_2_8, fact1_of_1_2_8.
+      assert (claim5 : isSubsetOf (Cl (union (AxmSet hs n) (insertion (Filter hs n) n))) (Cl (Cl (union (improveFilter (TH hs) n) (insertion (improveFilter (TH hs) n) n))))).
+      { transitivity (Cl (union (improveFilter (TH hs) n) (insertion (improveFilter (TH hs) n) n)))...
+        apply fact4_of_1_2_8.
+        intros b.
+        do 2 rewrite in_union_iff.
+        intros H1.
+        inversion H1; subst...
+      }
+      split...
+  Qed.
+
+  Lemma completeness_theorem_prototype :
+    forall hs : ensemble formula,
+    forall c : formula,
+    hs |= c ->
+    forall E : env,
+    equiconsistent (TH (insert (NegationF c) hs)) (eval_formula E) ->
+    isSubsetOf (TH (insert (NegationF c) hs)) (eval_formula E) ->
+    isFilter (eval_formula E) ->
+    hs |- c.
+  Proof with eauto with *.
+    intros hs c H_entail E.
+    set (v := eval_formula E).
+    intros H_equiconsistent H_incl H_isFilter.
+    assert (claim1 : inconsistent (TH (insert (NegationF c) hs))).
+    { apply H_equiconsistent.
+      enough (claim1_aux1 : inconsistent (Cl v))...
+      apply property1_of_inconsistent.
+      apply (ContradictionI c).
+      - apply ByAssumption.
+        enough (claim1_aux2 : satisfies E c) by now inversion claim1_aux2; subst.
+        apply H_entail.
+        intros h H.
+        constructor.
+        apply H_incl.
+        constructor.
+        apply ByAssumption, in_insert_iff...
+      - apply ByAssumption.
+        apply H_incl.
+        constructor.
+        apply ByAssumption, in_insert_iff...
+    }
+    assert (claim2 : inconsistent (Cl (insert (NegationF c) hs))).
+    { apply (inconsistent_isSubsetOf (TH (insert (NegationF c) hs)))...
+      apply TH_isSubsetOf_Cl.
+    }
+    apply NegationE, property1_of_inconsistent...
+  Qed.
+
+  Definition MaximalConsistentSet : ensemble formula -> ensemble formula :=
+    fun bs : ensemble formula =>
+    CompleteFilter (TH bs)
+  .
+
+  Inductive FullAxmSet : ensemble formula -> ensemble formula :=
+  | InFullAxmSet :
+    forall n : nat,
+    forall bs : ensemble formula,
+    forall b : formula,
+    member b (AxmSet bs n) ->
+    member b (FullAxmSet bs)
+  .
+
+  Local Hint Constructors FullAxmSet : core.
+
+  Lemma lemma2_of_1_3_9 :
+    forall bs : ensemble formula,
+    isSubsetOf (MaximalConsistentSet bs) (TH (FullAxmSet bs)).
+  Proof with eauto with *.
+    intros bs p H.
+    inversion H; subst.
+    assert (H1 := proj1 (lemma1_of_1_3_9 n bs) p H0).
+    inversion H1; subst.
+    constructor.
+    apply (extendInfers p H2)...
+  Qed.
+
+  Lemma lemma3_of_1_3_9_aux1 :
+    forall ps : list formula,
+    forall bs : ensemble formula,
+    (forall p : formula, In p ps -> member p (FullAxmSet bs)) ->
+    exists m : nat, (forall p : formula, In p ps -> member p (Filter bs m)).
+  Proof with eauto with *.
+    induction ps as [| p ps IH]; simpl.
+    - intros bs H.
+      exists 0...
+    - intros bs H.
+      assert (claim1 : forall h : formula, In h ps -> member h (FullAxmSet bs)) by firstorder.
+      assert (claim2 : member p (FullAxmSet bs)) by firstorder.
+      inversion claim2; subst.
+      assert (claim3 : member p (Filter bs n)).
+      { apply (proj2 (lemma1_of_1_3_9 n bs) p).
+        constructor.
+        apply ByAssumption...
+      }
+      destruct (IH bs claim1) as [n' H1].
+      destruct (le_lt_dec n' n) as [Hle | Hlt].
+      + exists n.
+        intros h [H2 | H2].
+        * subst...
+        * apply (lemma1_of_1_2_12  n' n Hle (TH bs))...
+      + exists n'.
+        intros h [H2 | H2]; subst.
+        * assert (H3 : n <= n') by lia.
+          apply (lemma1_of_1_2_12 n n' H3 (TH bs))...
+        * apply H1...
+  Qed.
+
+  Lemma lemma3_of_1_3_9 :
+    forall bs : ensemble formula,
+    isSubsetOf (TH (FullAxmSet bs)) (MaximalConsistentSet bs).
+  Proof with eauto with *.
+    intros bs p H.
+    inversion H; subst.
+    destruct (infers_has_compactness (FullAxmSet bs) p H0) as [ps [H1 [hs' [H2 H3]]]].
+    destruct (lemma3_of_1_3_9_aux1 ps bs H1) as [m H4].
+    assert (H5 : isFilter (improveFilter (TH bs) m)) by apply lemma1_of_1_2_11, lemma1_of_1_3_8.
+    assert (H6 := proj1 H5).
+    destruct (proj2 H5) as [H7 H8].
+    exists m.
+    apply (H7 (fold_right andB trueB ps) p).
+    - apply fact5_of_1_2_8.
+      + apply H5.
+      + exists ps...
+    - apply leq_LBA, (andBs_LBA ps hs')...
+      firstorder.
+  Qed.
+
+  Definition isMetaDN : ensemble formula -> Prop :=
+    fun bs : ensemble formula =>
+    forall p1 : formula,
+    (member (NegationF p1) bs -> member ContradictionF bs) ->
+    member p1 bs
+  .
+
+  Definition isImplicationFaithful : ensemble formula -> Prop :=
+    fun bs : ensemble formula =>
+    forall p1 : formula,
+    forall p2 : formula,
+    member (ImplicationF p1 p2) bs <-> (member p1 bs -> member p2 bs)
+  .
+
+  Lemma theorem_of_1_3_10_aux1 (bs : ensemble formula) :
+    isSubsetOf (TH bs) (MaximalConsistentSet bs).
+  Proof with eauto with *.
+    apply theorem_of_1_2_14...
+  Qed.
+
+  Lemma theorem_of_1_3_10_aux2 (bs : ensemble formula) :
+    equiconsistent (TH bs) (MaximalConsistentSet bs).
+  Proof with eauto with *.
+    apply lemma3_of_1_2_13...
+  Qed.
+
+  Lemma theorem_of_1_3_10_aux3 (bs : ensemble formula) :
+    forall p : formula,
+    member p (MaximalConsistentSet bs) <-> MaximalConsistentSet bs |- p.
+  Proof with eauto with *.
+    intros p.
+    split.
+    - intros H.
+      assert (claim1 : member p (TH (MaximalConsistentSet bs))) by now apply Cl_isSubsetOf_TH, fact3_of_1_2_8.
+      inversion claim1; subst...
+    - intros H.
+      apply fact5_of_1_2_8.
+      + apply theorem_of_1_2_14...
+      + apply TH_isSubsetOf_Cl...
+  Qed.
+
+  Theorem theorem_of_1_3_10 :
+    forall bs : ensemble formula,
+    isSubsetOf (TH bs) (MaximalConsistentSet bs) /\ equiconsistent (TH bs) (MaximalConsistentSet bs) /\ (forall p : formula, member p (MaximalConsistentSet bs) <-> MaximalConsistentSet bs |- p) /\ isMetaDN (MaximalConsistentSet bs) /\ isImplicationFaithful (MaximalConsistentSet bs).
+  Proof with eauto with *.
+    assert (lemma1 := @isSubsetOf_singleton formula).
+    assert (lemma2 : forall hs : ensemble formula, forall h : formula, isSubsetOf hs (insert h hs)).
+    { intros hs h b.
+      rewrite in_insert_iff...
+    }
+    assert (lemma3 := @isSubsetOf_empty formula).
+    assert (lemma4 : forall hs : ensemble formula, forall h : formula, member h (insert h hs)).
+    { intros hs h.
+      apply in_insert_iff...
+    }
+    intros bs.
+    assert (claim1 := theorem_of_1_3_10_aux1 bs).
+    assert (claim2 := theorem_of_1_3_10_aux2 bs).
+    assert (claim3 := theorem_of_1_3_10_aux3 bs).
+    assert (claim4 : isComplete (MaximalConsistentSet bs)) by apply theorem_of_1_2_14, lemma1_of_1_3_8.
+    assert (claim5 : isMetaDN (MaximalConsistentSet bs)).
+    { intros p1 H.
+      apply (claim4 p1).
+      split.
+      - apply inconsistent_isSubsetOf.
+        transitivity (insert p1 (MaximalConsistentSet bs))...
+      - intros H0.
+        assert (claim5_aux1 : insert p1 (MaximalConsistentSet bs) |- ContradictionF) by now apply property1_of_inconsistent.
+        exists ContradictionF.
+        split.
+        + apply H, claim3, NegationI...
+        + reflexivity.
+    }
+    assert (claim6 : isImplicationFaithful (MaximalConsistentSet bs)).
+    { intros p1 p2.
+      split.
+      - intros H H0.
+        apply claim3.
+        apply (ImplicationE p1 p2).
+        + apply claim3...
+        + apply claim3...
+      - intros H.
+        apply claim5.
+        intros H0.
+        apply claim3.
+        assert (claim6_aux1 : insert (ImplicationF p1 p2) (MaximalConsistentSet bs) |- ContradictionF).
+        { apply (ContradictionI (ImplicationF p1 p2)).
+          - apply ByAssumption, in_insert_iff, or_introl...
+          - apply (@extendInfers (MaximalConsistentSet bs) (NegationF (ImplicationF p1 p2))).
+            + apply claim3...
+            + apply lemma2.
+        }
+        assert (claim6_aux2 : MaximalConsistentSet bs |- ConjunctionF p1 (NegationF p2)).
+        { apply (DisjunctionE p1 (NegationF p1)).
+          - apply (extendInfers (DisjunctionF p1 (NegationF p1)) (Law_of_Exclusive_Middle p1))...
+          - apply (DisjunctionE p2 (NegationF p2)).
+            + apply (extendInfers (DisjunctionF p2 (NegationF p2)) (Law_of_Exclusive_Middle p2))...
+            + apply ContradictionE.
+              apply (cut_property (ImplicationF p1 p2)).
+              * apply ImplicationI.
+                apply ByAssumption.
+                apply in_insert_iff, or_intror, in_insert_iff, or_introl...
+              * apply (extendInfers ContradictionF claim6_aux1).
+                apply isSubsetOf_insert.
+                transitivity (insert p1 (MaximalConsistentSet bs))...
+            + apply ConjunctionI.
+              { apply ByAssumption.
+                apply in_insert_iff, or_intror, in_insert_iff, or_introl...
+              }
+              { apply (DisjunctionE p2 (NegationF p2)).
+                - apply (extendInfers (DisjunctionF p2 (NegationF p2)) (Law_of_Exclusive_Middle p2))...
+                - apply ContradictionE.
+                  apply (cut_property (ImplicationF p1 p2)).
+                  + apply ImplicationI.
+                    apply ByAssumption.
+                    apply in_insert_iff, or_intror, in_insert_iff, or_introl...
+                  + apply (extendInfers ContradictionF claim6_aux1).
+                    apply isSubsetOf_insert.
+                    transitivity (insert (NegationF p2) (insert p1 (MaximalConsistentSet bs))).
+                    * transitivity (insert p1 (MaximalConsistentSet bs))...
+                    * apply lemma2.
+                - apply ByAssumption...
+              }
+          - apply ContradictionE.
+            apply (cut_property (ImplicationF p1 p2)).
+            + apply ImplicationI.
+              apply ContradictionE.
+              apply (ContradictionI p1).
+              * apply ByAssumption...
+              * apply ByAssumption.
+                apply in_insert_iff, or_intror...
+            + apply (extendInfers ContradictionF claim6_aux1).
+              apply isSubsetOf_insert...
+        }
+      assert (claim6_aux3 : MaximalConsistentSet bs |- p1) by now apply (ConjunctionE1 p1 (NegationF p2)).
+      assert (claim6_aux4 : MaximalConsistentSet bs |- NegationF p2) by now apply (ConjunctionE2 p1 (NegationF p2)).
+      apply (ContradictionI p2).
+      + apply claim3, H, claim3...
+      + apply claim6_aux4.
+    }
+    tauto.
+  Qed.
+
+End PropertiesOfPropostionalLogic.
+
+Module SoundnessOfPL.
+
+  Import MyEnsemble MyEnsembleNova ClassicalLogic SyntaxOfPL SemanticsOfPL InferenceRulesOfPL.
+
+  Lemma ByAssumption_preserves {hs : ensemble formula} :
+    forall a : formula,
+    member a hs ->
+    hs |= a.
+  Proof with eauto with *.
+    intros c H.
+    apply (@extendEntails \left\{ c \right\} c)...
+  Qed.
+
+  Lemma ContradictionI_preserves {hs : ensemble formula} :
+    forall a : formula,
+    hs |= a ->
+    hs |= (NegationF a) ->
+    hs |= ContradictionF.
+  Proof with simpl in *; tauto.
+    intros a H H0 v H1.
+    assert (H2 := H v H1).
+    assert (H3 := H0 v H1).
+    inversion H2; subst.
+    inversion H3; subst...
+  Qed.
+
+  Lemma ContradictionE_preserves {hs : ensemble formula} :
+    forall a : formula,
+    hs |= ContradictionF ->
+    hs |= a.
+  Proof with simpl in *; tauto.
+    intros a H v H0.
+    assert (H1 := H v H0).
+    inversion H1; subst...
+  Qed.
+
+  Lemma NegationI_preserves {hs : ensemble formula} :
+    forall a : formula,
+    insert a hs |= ContradictionF ->
+    hs |= NegationF a.
+  Proof with simpl in *; tauto.
+    intros a H v H0.
+    constructor.
+    simpl.
+    intros H1.
+    assert (claim1 : forall h : formula, member h (insert a hs) -> satisfies v h).
+    { intros h.
+      rewrite in_insert_iff.
+      intros [H2 | H2]; constructor.
+      - rewrite H2...
+      - assert (H3 := H0 h H2).
+        inversion H3; subst...
+    }
+    assert (H2 := H v claim1).
+    inversion H2; subst...
+  Qed.
+
+  Lemma NegationE_preserves {hs : ensemble formula} :
+    forall a : formula,
+    insert (NegationF a) hs |= ContradictionF ->
+    hs |= a.
+  Proof with simpl in *; tauto.
+    intros a H v H0.
+    constructor.
+    apply NNPP.
+    intros H1.
+    assert (claim1 : forall h : formula, member h (insert (NegationF a) hs) -> satisfies v h).
+    { intros h.
+      rewrite in_insert_iff.
+      intros [H2 | H2]; constructor.
+      - rewrite H2...
+      - assert (H3 := H0 h H2).
+        inversion H3; subst...
+    }
+    assert (H2 := H v claim1).
+    inversion H2; subst...
+  Qed.
+
+  Lemma ConjunctionI_preserves {hs : ensemble formula} :
+    forall a : formula,
+    forall b : formula,
+    hs |= a ->
+    hs |= b ->
+    hs |= (ConjunctionF a b).
+  Proof with simpl in *; tauto.
+    intros a b H H0 v H1.
+    constructor.
+    assert (H2 := H v H1).
+    assert (H3 := H0 v H1).
+    inversion H2; subst.
+    inversion H3; subst...
+  Qed.
+
+  Lemma ConjunctionE1_preserves {hs : ensemble formula} :
+    forall a : formula,
+    forall b : formula,
+    hs |= ConjunctionF a b ->
+    hs |= a.
+  Proof with simpl in *; tauto.
+    intros a b H v H0.
+    constructor.
+    assert (H1 := H v H0).
+    inversion H1; subst...
+  Qed.
+
+  Lemma ConjunctionE2_preserves {hs : ensemble formula} :
+    forall a : formula,
+    forall b : formula,
+    hs |= ConjunctionF a b ->
+    hs |= b.
+  Proof with simpl in *; tauto.
+    intros a b H v H0.
+    constructor.
+    assert (H1 := H v H0).
+    inversion H1; subst...
+  Qed.
+
+  Lemma DisjunctionI1_preserves {hs : ensemble formula} :
+    forall a : formula,
+    forall b : formula,
+    hs |= a ->
+    hs |= DisjunctionF a b.
+  Proof with simpl in *; tauto.
+    intros a b H v H0.
+    constructor.
+    assert (H1 := H v H0).
+    inversion H1; subst...
+  Qed.
+
+  Lemma DisjunctionI2_preserves {hs : ensemble formula} :
+    forall a : formula,
+    forall b : formula,
+    hs |= b ->
+    hs |= DisjunctionF a b.
+  Proof with simpl in *; tauto.
+    intros a b H v H0.
+    constructor.
+    assert (H1 := H v H0).
+    inversion H1; subst...
+  Qed.
+
+  Lemma DisjunctionE_preserves {hs : ensemble formula} :
+    forall a : formula,
+    forall b : formula,
+    forall c : formula,
+    hs |= DisjunctionF a b ->
+    insert a hs |= c ->
+    insert b hs |= c ->
+    hs |= c.
+  Proof with simpl in *; tauto.
+    intros a b c H H0 H1 v H2.
+    constructor.
+    assert (H3 := H v H2).
+    inversion H3; subst.
+    destruct H4 as [H4 | H4].
+    - assert (claim1 : forall h : formula, member h (insert a hs) -> satisfies v h).
+      { intros h.
+        rewrite in_insert_iff.
+        intros [H5 | H5]; constructor.
+        - rewrite H5...
+        - assert (H6 := H2 h H5).
+          inversion H6; subst...
+      }
+      assert (H5 := H0 v claim1).
+      inversion H5; subst...
+    - assert (claim1 : forall h : formula, member h (insert b hs) -> satisfies v h).
+      { intros h.
+        rewrite in_insert_iff.
+        intros [H5 | H5]; constructor.
+        - rewrite H5...
+        - assert (H6 := H2 h H5).
+          inversion H6; subst...
+      }
+      assert (H5 := H1 v claim1).
+      inversion H5; subst...
+  Qed.
+
+  Lemma ImplicationI_preserves {hs : ensemble formula} :
+    forall a : formula,
+    forall b : formula,
+    insert a hs |= b ->
+    hs |= ImplicationF a b.
+  Proof with simpl in *; tauto.
+    intros a b H v H0.
+    constructor.
+    simpl.
+    intros H1.
+    assert (claim1 : forall h : formula, member h (insert a hs) -> satisfies v h).
+    { intros h.
+      rewrite in_insert_iff.
+      intros [H2 | H2]; constructor.
+      - rewrite H2...
+      - assert (H3 := H0 h H2).
+        inversion H3; subst...
+    }
+    assert (H2 := H v claim1).
+    inversion H2; subst...
+  Qed.
+
+  Lemma ImplicationE_preserves {hs : ensemble formula} :
+    forall a : formula,
+    forall b : formula,
+    hs |= ImplicationF a b ->
+    hs |= a ->
+    hs |= b.
+  Proof with simpl in *; tauto.
+    intros a b H H0 v H1.
+    constructor.
+    assert (H2 := H v H1).
+    inversion H2; subst.
+    simpl in H3.
+    apply H3.
+    assert (H4 := H0 v H1).
+    inversion H4; subst...
+  Qed.
+
+  Lemma BiconditionalI_preserves {hs : ensemble formula} :
+    forall a : formula,
+    forall b : formula,
+    insert a hs |= b ->
+    insert b hs |= a ->
+    hs |= BiconditionalF a b.
+  Proof with simpl in *; tauto.
+    intros a b H H0 v H1.
+    constructor.
+    simpl.
+    split.
+    - intros H2.
+      assert (claim1 : forall h : formula, member h (insert a hs) -> satisfies v h).
+      { intros h.
+        rewrite in_insert_iff.
+        intros [H3 | H3]; constructor.
+        - rewrite H3...
+        - assert (H4 := H1 h H3).
+          inversion H4; subst...
+      }
+      assert (H3 := H v claim1).
+      inversion H3; subst...
+    - intros H2.
+      assert (claim1 : forall h : formula, member h (insert b hs) -> satisfies v h).
+      { intros h.
+        rewrite in_insert_iff.
+        intros [H3 | H3]; constructor.
+        - rewrite H3...
+        - assert (H4 := H1 h H3).
+          inversion H4; subst...
+      }
+      assert (H3 := H0 v claim1).
+      inversion H3; subst...
+  Qed.
+
+  Lemma BiconditionalE1_preserves {hs : ensemble formula} :
+    forall a : formula,
+    forall b : formula,
+    hs |= BiconditionalF a b ->
+    hs |= a ->
+    hs |= b.
+  Proof with simpl in *; tauto.
+    intros a b H H0 v H1.
+    constructor.
+    assert (H2 := H v H1).
+    inversion H2; subst.
+    simpl in H3.
+    apply (proj1 H3).
+    assert (H4 := H0 v H1).
+    inversion H4; subst...
+  Qed.
+
+  Lemma BiconditionalE2_preserves {hs : ensemble formula} :
+    forall a : formula,
+    forall b : formula,
+    hs |= BiconditionalF a b ->
+    hs |= b ->
+    hs |= a.
+  Proof with simpl in *; tauto.
+    intros a b H H0 v H1.
+    constructor.
+    assert (H2 := H v H1).
+    inversion H2; subst.
+    simpl in H3.
+    apply (proj2 H3).
+    assert (H4 := H0 v H1).
+    inversion H4; subst...
+  Qed.
+
+  Theorem Soundness (hs : ensemble formula) (c : formula) (_infer : hs |- c) :
+    hs |= c.
+  Proof with firstorder.
+    induction _infer.
+    - apply (ByAssumption_preserves h)...
+    - apply (ContradictionI_preserves a)...
+    - apply (ContradictionE_preserves a)...
+    - apply (NegationI_preserves a)...
+    - apply (NegationE_preserves a)...
+    - apply (ConjunctionI_preserves a b)...
+    - apply (ConjunctionE1_preserves a b)...
+    - apply (ConjunctionE2_preserves a b)...
+    - apply (DisjunctionI1_preserves a b)...
+    - apply (DisjunctionI2_preserves a b)...
+    - apply (DisjunctionE_preserves a b c)...
+    - apply (ImplicationI_preserves a b)...
+    - apply (ImplicationE_preserves a b)...
+    - apply (BiconditionalI_preserves a b)...
+    - apply (BiconditionalE1_preserves a b)...
+    - apply (BiconditionalE2_preserves a b)...
+  Qed.
+
+End SoundnessOfPL.
+
+Module CompletenessOfPL.
+
+  Import ListNotations BasicSetoidTheory MyEnsemble BasicPosetTheory MyEnsembleNova CountableBooleanAlgebra ClassicalLogic SyntaxOfPL SemanticsOfPL InferenceRulesOfPL LindenbaumBooleanAlgebraOnPL PropertiesOfPropostionalLogic SoundnessOfPL.
+
+  Variant makeEnv (bs : ensemble formula) (i : pvar) : value :=
+  | pos_pvar : member (AtomF i) bs -> makeEnv bs i
+  | neg_pvar : ~ member (AtomF i) bs -> makeEnv bs i
+  .
+
+  Parameter ModelExistsIfConsistent : forall hs : ensemble formula, ~ hs |- ContradictionF -> MaximalConsistentSet hs == eval_formula (makeEnv (MaximalConsistentSet hs)).
+
+  Corollary Completeness :
+    forall hs : ensemble formula,
+    forall c : formula,
+    hs |= c ->
+    hs |- c.
+  Proof with try now firstorder.
+    intros hs c H_entail.
+    destruct (classic (hs |- c)) as [H_yes | H_no].
+    - apply H_yes.
+    - assert (claim1 : ~ insert (NegationF c) hs |- ContradictionF).
+      { intros H_impossible.
+        apply H_no, NegationE...
+      }
+      assert (claim2 : isFilter (MaximalConsistentSet (insert (NegationF c) hs))) by apply theorem_of_1_2_14, lemma1_of_1_3_8.
+      assert (H_eq := ModelExistsIfConsistent (insert (NegationF c) hs) claim1).
+      apply (completeness_theorem_prototype hs c H_entail (makeEnv (MaximalConsistentSet (insert (NegationF c) hs)))).
+      + unfold equiconsistent.
+        transitivity (inconsistent (MaximalConsistentSet (insert (NegationF c) hs))).
+        * apply theorem_of_1_3_10.
+        * split; apply inconsistent_isSubsetOf...
+      + transitivity (MaximalConsistentSet (insert (NegationF c) hs)).
+        * apply theorem_of_1_3_10.
+        * firstorder.
+      + apply (isFilter_ext_eq (MaximalConsistentSet (insert (NegationF c) hs)) claim2)...
+  Qed.
+
+End CompletenessOfPL.
