README.md
@@ -28,8 +28,7 @@ coqc -Q . DschingisKhan pure/MyCoin.v
 coqc -Q . DschingisKhan classical/ExclusiveMiddle.v
 coqc -Q . DschingisKhan classical/DomainTheory.v
 coqc -Q . DschingisKhan projects/PropositionalLogic/Basics.v
-coqc -Q . DschingisKhan projects/PropositionalLogic/Soundness.v
-coqc -Q . DschingisKhan projects/PropositionalLogic/Completeness.v
+coqc -Q . DschingisKhan projects/PropositionalLogic/MetaTheorems.v
 coqc -Q . DschingisKhan projects/PropositionalLogic.v
 coqc -Q . DschingisKhan projects/SmullyanGIT/Chapter1.v
 coqc -Q . DschingisKhan projects/SmullyanGIT.v
